# SPDX-License-Identifier: GPL-3.0-or-later	

@base             <http://purl.org/oseg/ontologies/OTRL> .
@prefix owl:      <http://www.w3.org/2002/07/owl#> .
@prefix rdf:      <http://www.w3.org/1999/02/22-rdf-syntax-ns#> .
@prefix rdfs:     <http://www.w3.org/2000/01/rdf-schema#> .

<>
  a owl:Ontology ;
  owl:versionInfo "1.0" ;
  owl:versionIRI <> ;
  rdfs:label "TLR for OSH meta data"@en ;
  rdfs:comment "Technology Readiness Level can be used to assess the project stage of Open Source Hardware"@en ;
  terms:contributor "Martin HÃ¤uer <martin.haeuer@ose-germany.de>" ;
  terms:contributor "Robin Vobruba <hoijui.quaero@gmail.com>" ;
  terms:license "GPL-3.0-or-later" .

# properties & classes: (description from NASA are used under public domain)

:OTRL
  a owl:class ;
  rdfs:label "open TLR"@en ;
  rdfs:comment "Technology Readiness Level for open source hardware; labels are used from EU-H2020 https://ec.europa.eu/research/participants/data/ref/h2020/other/wp/2016-2017/annexes/h2020-wp1617-annex-ga_en.pdf"@en ;
  # That's the main class then!
  .

:ODRL
  a owl:class ;
  rdfs:label "open DLR"@en ;
  rdfs:comment "Documentation Readiness Level for open source hardware"@en ;
  # That's the main class then!
  .

:hardwareDescription
  a owl:DatatypeProperty ;
  rdfs:label "hardware description"@en ;
  rdfs:comment "Hardware-specific description of this OTRL; inspired by: https://www.nasa.gov/pdf/458490main_TRL_Definitions.pdf"@en ;
  rdfs:range schema:Text ;
  owl:cardinality 1 ;
  rdfs:domain :OTRL ;
  .

:softwareDescription
  a owl:DatatypeProperty ;
  rdfs:label "software description"@en ;
  rdfs:comment "Software-specific description of this OTRL; inspired by: https://www.nasa.gov/pdf/458490main_TRL_Definitions.pdf"@en ;
  rdfs:range schema:Text ;
  owl:cardinality 1 ;
  rdfs:domain :OTRL ;
  .

:documentationDescription
  a owl:DatatypeProperty ;
  rdfs:label "documentation description"@en ;
  rdfs:comment "required state of the documentation for this OTRL"@en ;
  rdfs:range schema:Text ;
  owl:cardinality 1 ;
  rdfs:domain :OTRL ;
  .

:exitCriteria
  a owl:DatatypeProperty ;
  rdfs:label "Exit criteria"@en ;
  rdfs:comment "Criteria to exit this OTRL for the next OTRL; inspired by: https://www.nasa.gov/pdf/458490main_TRL_Definitions.pdf"@en ;
  rdfs:range schema:Text ;
  owl:cardinality 1 ;
  rdfs:domain :OTRL ;
  .

# the technology readiness levels (TLR):

:OTRL-1
  a owl:class ;
  rdfs:subClassOf :OTRL ;
  rdfs:label "OTRL-1"@en ;
  rdfs:comment "Basic principles observed"@en ;
  :hardwareDescription "Knowledge generated underpinning hardware technology concepts/applications."@en ;
  :softwareDescription "Knowledge generated underpinning basic properties of software architecture and mathematical formulation."@en ;
  :exitCriteria "The proposed concept/application is documented in feasible manner and published under a free/open license."@en ;
  .

:OTRL-2
  a owl:class ;
  rdfs:subClassOf :OTRL ;
  rdfs:label "OTRL-2"@en ;
  rdfs:comment "Technology concept formulated"@en ;
  :hardwareDescription "Invention begins, practical application is identified but is speculative, no experimental proof (e.g. a physical prototype) or detailed analysis is available yet to support the conjecture."@en ;
  :softwareDescription "Basic principles coded. Experiments performed with synthetic data. Practical application is identified but is speculative, no experimental proof or detailed analysis is available yet to support the conjecture."@en ;
  :exitCriteria "A more detailled description of the concept/application that addresses feasibility and benefit is documented in feasible manner and published under a free/open license."@en ;
  .

:OTRL-3
  a owl:class ;
  rdfs:subClassOf :OTRL ;
  rdfs:label "OTRL-3"@en ;
  rdfs:comment "Experimental proof of concept"@en ;
  :hardwareDescription "Key functions of the concept tested & proven in a controlled environment (e.g. laboratory)"@en ;
  :softwareDescription "Development of limited functionality to validate critical properties and predictions using non-integrated software components."@en ;
  :exitCriteria "Practically applied concept (e.g. conceptional prototype) and validating test results are documented in feasible manner and published under a free/open license."@en ;
  .

:OTRL-4
  a owl:class ;
  rdfs:subClassOf :OTRL ;
  rdfs:label "OTRL-4"@en ;
  rdfs:comment "Technology validated in lab"@en ;
  :hardwareDescription "A low fidelity application (prototype) was built and operated in a controlled environment (e.g. laboratory) demonstrating basic functionality and critical test environments; performance predictions are formulated towards the final operating environment."@en ;
  :softwareDescription "Key functionally and critical software components are integrated, and functionally validated, to establish interoperability and begin architecture development. Relevant Environments defined and performance in this environment predicted."@en ;
  :exitCriteria "Prototype, validating test results and definition of relevant application environment are documented in feasible manner and published under a free/open license."@en ;
  .

:OTRL-5
  a owl:class ;
  rdfs:subClassOf :OTRL ;
  rdfs:label "OTRL-5"@en ;
  rdfs:comment "Technology validated in relevant environment"@en ;
  :hardwareDescription "A medium fidelity system/component brassboard is built and operated to demonstrate overall performance in a simulated operational environment with realistic support elements that demonstrates overall performance in critical areas. Performance predictions are made for subsequent development phases."@en ;
  :softwareDescription "ToDo"@en ;
  :exitCriteria "ToDo"@en ;
  .

:OTRL-6
  a owl:class ;
  rdfs:subClassOf :OTRL ;
  rdfs:label "OTRL-6"@en ;
  rdfs:comment "Technology demonstrated in relevant environment"@en ;
  :hardwareDescription "A high fidelity system/component prototype that adequately addresses all critical scaling issues is built and operated in a relevant environment to demonstrate operations under critical environmental conditions."@en ;
  :softwareDescription "ToDo"@en ;
  :exitCriteria "ToDo"@en ;
  .

:OTRL-7
  a owl:class ;
  rdfs:subClassOf :OTRL ;
  rdfs:label "OTRL-7"@en ;
  rdfs:comment "System prototype demonstration in operational environment"@en ;
  :hardwareDescription "A high fidelity engineering unit that adequately addresses all critical scaling issues is built and operated in a relevant environment to demonstrate performance in the actual operational environment and platform (ground, airborne, or space)."@en ;
  :softwareDescription "ToDo"@en ;
  :exitCriteria "ToDo"@en ;
  .

:OTRL-8
  a owl:class ;
  rdfs:subClassOf :OTRL ;
  rdfs:label "OTRL-8"@en ;
  rdfs:comment "System complete and qualified"@en ;
  :hardwareDescription "Hardware, in its final version, has been built and operated in the intended operational environment and proven its performance. All documentation has been completed."@en ;
  :softwareDescription "All software has been thoroughly debugged and fully integrated with all operational hardware and software systems. All user documentation, training documentation, and maintenance documentation completed. All functionality successfully demonstrated in simulated operational scenarios. Documentatoin."@en ;
  :exitCriteria "ToDo"@en ;
  .

:OTRL-9
  a owl:class ;
  rdfs:subClassOf :OTRL ;
  rdfs:label "OTRL-9"@en ;
  rdfs:comment "Actual system proven in operational environment (e.g. production by multiple stakeholders)"@en ;
  :hardwareDescription "Hardware has been _independently_ built and operated in the final operational environment and proven its performance."@en ;
  :softwareDescription "Software is replicated, integrated and operated _independently_ in the final operational hardware/software systems and proven its performance."@en ;
  .

:ODRL-0
  a owl:class ;
  rdfs:subClassOf :ODRL ;
  rdfs:label "ODRL-1"@en ;
  rdfs:comment "no documentation available"@en ;
  .

:ODRL-1
  a owl:class ;
  rdfs:subClassOf :ODRL ;
  rdfs:label "ODRL-1"@en ;
  rdfs:comment "basic information available"@en ;
  .

:ODRL-2
  a owl:class ;
  rdfs:subClassOf :ODRL ;
  rdfs:label "ODRL-2"@en ;
  rdfs:comment "drafty documentation"@en ;
  .

:ODRL-3
  a owl:class ;
  rdfs:subClassOf :ODRL ;
  rdfs:label "ODRL-3"@en ;
  rdfs:comment "early release"@en ;
  .

:ODRL-4
  a owl:class ;
  rdfs:subClassOf :ODRL ;
  rdfs:label "ODRL-4"@en ;
  rdfs:comment "relevant release"@en ;
  .

:ODRL-5
  a owl:class ;
  rdfs:subClassOf :ODRL ;
  rdfs:label "ODRL-5"@en ;
  rdfs:comment "mature release"@en ;
  .